Splinter/Betree/Buffer.i.dfy
@@ -1,0 +1,34 @@
+// Copyright 2018-2021 VMware, Inc., Microsoft Inc., Carnegie Mellon University, ETH Zurich, and University of Washington
+// SPDX-License-Identifier: BSD-2-Clause
+
+include "../../lib/Base/KeyType.s.dfy"
+include "../../Spec/Message.s.dfy"
+
+module BufferMod
+{
+  import opened KeyType
+  import opened ValueMessage
+
+  predicate AnyKey(key: Key) { true }
+  predicate Total(keys: iset<Key>) {
+    forall k | AnyKey(k) :: k in keys
+  }
+  function AllKeys() : (out: iset<Key>)
+    ensures Total(out)
+  {
+    iset k | AnyKey(k)
+  }
+
+  datatype Buffer = Buffer(mapp: map<Key, Message>)
+  {
+    function Query(key: Key) : Message
+    {
+      if key in mapp then mapp[key] else Update(NopDelta())
+    }
+
+    function ApplyFilter(accept: iset<Key>) : Buffer
+    {
+      Buffer(map k | k in mapp && k in accept :: mapp[k])
+    }
+  }
+}
