Splinter/Betree/LinkedBufferStack.i.dfy
@@ -1,0 +1,116 @@
+// Copyright 2018-2021 VMware, Inc., Microsoft Inc., Carnegie Mellon University, ETH Zurich, and University of Washington
+// SPDX-License-Identifier: BSD-2-Clause
+
+include "../Disk/GenericDisk.i.dfy"
+include "BufferStack.i.dfy"
+  
+  
+module LinkedBufferStackMod {
+  import opened GenericDisk
+  import opened Maps
+  import opened KeyType
+  import opened ValueMessage
+  import opened BufferMod
+
+
+  // Note that this BufferStack is a pointer-y structure. It is different from
+  // Buffers.BufferStack
+  datatype BufferStack = BufferStack(buffers: seq<Address>)
+  {
+    predicate Valid(dv: BufferDiskView)
+    {
+      forall i:nat | i < |buffers| :: buffers[i] in dv.Addresses()
+    }
+
+    function Length() : nat 
+    {
+      |buffers|
+    }
+
+    function Slice(start: nat, end: nat) : BufferStack
+      requires start <= end <= |buffers|
+    {
+      BufferStack(buffers[start..end])
+    }
+
+    // function GetBuffer(addr: Address) : Buffers.Buffer
+    //   requires addr in buffers
+    // {
+    //   dv.Get(addr)
+    // }
+
+    function QueryUpTo(dv: BufferDiskView, key: Key, count: nat) : Message
+      requires count <= |buffers|
+      requires Valid(dv)
+    {
+      if count == 0 then Update(NopDelta())
+      else
+        Merge(QueryUpTo(dv, key, count-1), dv.Get(buffers[count-1]).Query(key))
+    }
+
+    function Query(dv: BufferDiskView, key: Key) : Message
+      requires Valid(dv)
+    {
+      QueryUpTo(dv, key, |buffers|)
+    }
+    
+    // TODO: compact equivalence needs this to validate 
+    // function ApplyFilter(accept: iset<Key>) : BufferStack
+    // {
+    //   BufferStack(seq(|buffers|, i requires 0<=i<|buffers| => buffers[i].ApplyFilter(accept)))
+    // }
+
+    function PushBufferStack(newBuffers: BufferStack) : BufferStack
+    {
+      BufferStack(newBuffers.buffers + this.buffers)
+    }
+
+    predicate Equivalent(dv: BufferDiskView, other: BufferStack)
+      requires Valid(dv)
+      requires other.Valid(dv)
+    {
+      forall k | AnyKey(k) :: Query(dv, k) == other.Query(dv, k)
+    }
+  }  // end type BufferStack
+
+
+    // move to different module
+  datatype BufferDiskView = BufferDiskView(entries: map<Address, Buffer>)
+  {
+    function Addresses() : set<Address>
+    {
+      entries.Keys
+    }
+
+    function Get(addr: Address) : Buffer
+      requires addr in entries
+    {
+      entries[addr]
+    }
+
+    function ModifyDisk(addr: Address, item: Buffer) : BufferDiskView {
+      BufferDiskView.BufferDiskView(entries[addr := item])
+    }
+
+    predicate IsSubDisk(bigger: BufferDiskView)
+    {
+      IsSubMap(entries, bigger.entries)
+    }
+
+    function {:opaque} MergeDisk(other: BufferDiskView) : (out: BufferDiskView)
+      // ensure result is sound -- keys and their values must come from one of these places
+      ensures forall addr | addr in out.entries 
+        :: || (addr in entries && out.entries[addr] == entries[addr])
+           || (addr in other.entries && out.entries[addr] == other.entries[addr])
+      // ensure result is complete -- result must contain all the keys
+      ensures entries.Keys <= out.entries.Keys
+      ensures other.entries.Keys <= out.entries.Keys
+    {
+      BufferDiskView(MapUnion(entries, other.entries))
+    }
+  }
+
+  function EmptyBufferDisk() : BufferDiskView {
+    BufferDiskView(map[])
+  }
+}
